FraudProof/Games/Base/LogProof.lean
@@ -1,0 +1,69 @@
+import FraudProof.Games.GameDef -- Players, Winner
+import FraudProof.Games.Base.GenericTree -- Generic Game trees
+import FraudProof.Games.Base.ElemInTree -- Linear basic game definition
+import FraudProof.Games.Base.LogarithmicTransformation
+
+import FraudProof.DataStructures.Sequence
+
+-- Non-emtpy path to generate complete perfect tree
+@[simp]
+def toTreeSeq (lgn : Nat) := Sequence (2^lgn.succ - 1)
+
+def skeleton_arena {lgn : Nat}
+  (skl : toTreeSeq lgn SkElem)
+  : ABTree SkElem Unit
+  := ABTree.map id (fun _ => ())
+  $ perfectSeq skl
+
+-- One follows side
+def get_spine {α : Type} (side : SkElem)( e : α × α ) : α
+  := match side with
+     | .inl _ => e.1
+     | .inr _ => e.2
+-- the other one the opposite
+def get_sibling {α : Type} (side : SkElem)( e : α × α ) : α
+  := match side with
+     | .inl _ => e.2
+     | .inr _ => e.1
+
+-- Extracting from proposer
+def extract_intermed_hashes {ℍ : Type}{n : Nat}
+  (skl : Sequence n SkElem) (prop : Sequence n (ℍ × ℍ))
+  : Sequence n ℍ
+  := seq_zip_with get_spine skl prop
+
+def extract_sibling_hashes {ℍ : Type}{n : Nat}
+  (skl : Sequence n SkElem) (prop : Sequence n (ℍ × ℍ))
+  : Sequence n ℍ
+  := seq_zip_with get_sibling skl prop
+
+-- Fussioning everything together here are all triangles such that
+-- proposer says
+-- (a , b , c) {side} := op_side side a c = b
+def gen_triangles {ℍ : Type}{n : Nat}{nNZ : 0 < n}
+  (skl : Sequence n SkElem)
+  (top_hash : ℍ)
+  (hashes : Sequence n (ℍ × ℍ))
+  : Sequence n (ℍ × ℍ × ℍ)
+  :=
+  have spine : Sequence n ℍ := extract_intermed_hashes skl hashes
+  have tupled_interval : Sequence n (ℍ × ℍ)
+    := seq_zip_with (fun a b => (a,b)) spine
+      (sequence_coerce (by apply Nat.succ_pred_eq_of_pos; assumption)
+      $ Fin.snoc (tailSeq' spine) top_hash)
+  seq_zip_with (fun (a,b) c => (a,b,c)) tupled_interval (extract_sibling_hashes skl hashes)
+
+def triangles_tree_to_range {ℍ : Type}
+  : ABTree (ℍ × ℍ × ℍ) (ℍ × ℍ × ℍ) -> ABTree ℍ (Range ℍ × Range ℍ)
+  | .leaf (_ , _ , sib) => .leaf sib
+  | .node (_ , mid, _ ) nleft nright => _
+
+-- def proposer_transformation {ℍ : Type}{lgn:Nat}
+--     (top_hash : ℍ)
+--     (skl : Sequence (2^lgn.succ - 2)  SkElem)
+--     (hashes : Sequence (2^lgn.succ - 2) (ℍ × ℍ))
+--     : ABTree ℍ ℍ
+--     := have spine : Sequence (2^lgn.succ - 1) ℍ
+--             := sequence_coerce (by simp; sorry )
+--                $ Fin.snoc (extract_intermed_hashes skl hashes) top_hash
+--     perfectSeq spine
